Add base.{base_,}interp_beq
These are the canonical boolean equality functions for the interpretations of the various base types.  This will probably come in handy for side conditions in proofs about reifications of rewrite rules.

src/Language.v
@@ -315,6 +315,23 @@ Module Compilers.
          | type.option A => Datatypes.option (interp A)
          end%type.
 
+    Fixpoint base_interp_beq {t} : base_interp t -> base_interp t -> bool
+      := match t with
+         | type.unit => fun _ _ => true
+         | type.Z => Z.eqb
+         | type.bool => Bool.eqb
+         | type.nat => Nat.eqb
+         | type.zrange => zrange_beq
+         end.
+
+    Fixpoint interp_beq {t} : interp t -> interp t -> bool
+      := match t with
+         | type.type_base t => @base_interp_beq t
+         | type.prod A B => prod_beq _ _ (@interp_beq A) (@interp_beq B)
+         | type.list A => list_beq _ (@interp_beq A)
+         | type.option A => option_beq (@interp_beq A)
+         end.
+
     Definition try_make_base_transport_cps
                (P : type.base -> Type) (t1 t2 : type.base)
       : ~> option (P t1 -> P t2)
